EvmCompiler/TypedCfg/Typing.lean
@@ -42,6 +42,8 @@ def type? (instr : Instr) (shape : Shape) : Option Shape :=
         | [], _ => none
       else
         none
+  | .relabel target =>
+      if shape.relabelCompatible target then some target else none
   | .unwind target =>
       Shape.unwindTo target shape
 
